<?xml version="1.0" encoding="UTF-8" ?>
<!-- =================================================================================================== -->
<!-- To process this file with xsltproc do                                                        -->
<!--                                                                                              -->
<!-- (1) LaTeX/PDF:                                                                               -->
<!--     xsltproc -o minimal.tex PATH_TO/mathbook/xsl/pretext-latex.xsl source/main.ptx           -->
<!--     pdflatex minimal.tex                                                                     -->
<!--     xelatex minimal.tex                                                                      -->
<!--                                                                                              -->
<!-- (2) HTML:                                                                                    -->
<!--     xsltproc PATH_TO/mathbook/xsl/pretext-html.xsl source/main.ptx                           -->
<!--     <browser>  minimal.html                                                                  -->
<!--        ~/xsltproc/xsltproc.exe ~/mathbook/xsl/mathbook-html.xsl test.xml                     -->
<!--                                                                                              -->
<!-- (3) CoCalc worksheet (parameter causes a single file for output)                             -->
<!--     REMOVE the "X" in the double dash (which is not legal in an XML comment)                 -->
<!--     xsltproc -X-stringparam chunk.level 0 PATH_TO/mathbook/xsl/pretext-smc.xsl source/main.ptx   -->
<!--     <CoCalc> minimal.sagews                                                                  -->
<!--                                                                                              -->
<!-- (4) Sage doctesting                                                                          -->
<!--     REMOVE the "X" in the double dash (which is not legal in an XML comment)                 -->
<!--     xsltproc -X-stringparam chunk.level 0 PATH_TO/mathbook/xsl/pretext-sage-doctest.xsl source/main.ptx  -->
<!--     <read further instructions in> minimal.py                                                -->
<!-- =================================================================================================== -->

<chapter xml:id="Calculus_2">



<!-- =================================================================================================== -->
<!-- Title and Other Preliminaries -->
<!-- =================================================================================================== -->
        <title>Taylor Series</title>

        <!-- <frontmatter> -->

<!--             <titlepage>
                <author>
                    <institution>University of Newcastle</institution>
                </author>
                <date><today /></date>
            </titlepage> -->

            <!-- <abstract>
                <p>This is a very short article, but it still exercises some advanced features of MathBook XML.</p>
            </abstract> -->

        <!-- </frontmatter> -->

        <!-- <introduction>
            <p>This is a short paragraph to introduce the article (but it is not the abstract).  It is optional, in case it would be preferable to have the first section be titled an <q>Introduction.</q></p>
        </introduction> -->
<!-- =================================================================================================== -->




<!-- =================================================================================================== -->
<!-- Section 1: Partial Differentiation -->
<!-- =================================================================================================== -->
        <section xml:id="Generating-New-Series-from-Known-Series">
            <title>Generating New Series from Known Series</title>
            <p>In Table <m>1</m> below we have listed the Maclaurin series for a small set of basic functions of science and engineering. These series can all be relatively easily derived from first principals as discussed in previous lectures. However, for some more complex functions it is easier to find their Maclaurin series by starting from known series rather than trying to find the series from scratch. We will look at two commonly used techniques.</p>
 
            
<p >
<ol >
<li >  Manipulating/Substituting into known series. </li >
<li >
<p >
Differentiating/Integrating known series.
</p >
</li >
</ol >
</p >           


 <p > <title> Some Important Maclaurin Series </title> </p>
 <p >
<ol >
<li >  <m> \dfrac{1}{1-x}=\sum_{k=0}^{\infty}x^{k}=1+x+x^{2}+x^{3}+\cdots . \hspace{5cm}  \lvert x\rvert &lt; 1  </m> </li >
<li >
<p >
<m> e^{x}=\sum_{k=0}^{\infty}\dfrac{x^{k}}{k!}=1+x+\dfrac{x^{2}}{2!} +\dfrac{x^{3}}{3!}+\cdots .  \hspace{5.6cm}\sim </m>
</p >
</li >
 <li >
<p >
<m> \sin(x)=\sum_{k=0}^{\infty}(-1)^{k}\dfrac{x^{2k+1}}{(2k+1)!}=x-\dfrac{x^{3}}{3!} +\dfrac{x^{5}}{5!}-\cdots .\hspace{3cm}\sim </m>
</p >
</li >
 <li >
<p >
<m> \cos(x)=\sum_{k=0}^{\infty}(-1)^{k}\dfrac{x^{2k}}{(2k)!}=1-\dfrac{x^{2}}{2!} +\dfrac{x^{4}}{4!}-\cdots .\hspace{3.9cm} \sim </m>
</p >
</li >
 <li >
<p >
<m> \ln(1+x)=\sum_{k=0}^{\infty}(-1)^{k-1}\dfrac{x^{k}}{(k)}=x-\dfrac{x^{2}}{2} +\dfrac{x^{3}}{3}-\cdots . \hspace{2.5cm}  \lvert x\rvert &lt; 1 </m>
</p >
</li >
<li >
<p >
<m> \tan^{-1}(1+x)=\sum_{k=0}^{\infty}(-1)^{k}\dfrac{x^{2k+1}}{(2k+1)}=x-\dfrac{x^{3}}{3} +\dfrac{x^{5}}{5}-\cdots . \hspace{1.1cm} \lvert x\rvert &lt; 1 </m>
</p >
</li >
 <li >
<p >
<m> \sinh(x)=\sum_{k=0}^{\infty}\dfrac{x^{2k+1}}{(2k+1)!}=x+\dfrac{x^{3}}{3!} +\dfrac{x^{5}}{5!}+\cdots . \hspace{3.9cm} \sim </m>
</p >
</li >
<li >
<p >
<m> \cosh(x)=\sum_{k=0}^{\infty}\dfrac{x^{2k}}{(2k)!}=1+\dfrac{x^{2}}{2!} +\dfrac{x^{4}}{4!}+\cdots . \hspace{4.8cm} \sim </m>
</p >
</li >
</ol >
</p >      
            
<paragraphs><title>Manipulating/Substituting into Known Series</title></paragraphs>

<example xml:id="Maclaurin_series_1_on_1_plus_x2">

            <p>Find the Maclaurin series for  <m> f(x)=\dfrac{1}{1+x^{2}}. </m> </p>
             <solution>
                    <p>We know that the Maclaurin series for<m>f(x)=\dfrac{1}{1-x}</m> on <m>\lvert x\rvert &lt; 1 </m> is </p>
                    
                    <me>  \dfrac{1}{1-x}=\sum_{k=0}^{\infty}x^{k}=1+x+x^{2}+x^{3}+\cdots \cdot </me>
                    <p>We can use this series by replacing <m> x </m> with <m> -x^{2} </m> to obtain </p>
                     <p><md>
                        <mrow>\dfrac{1}{1+x^{2}} \amp =\dfrac{1}{1-(-x^{2})}</mrow>
                        <mrow> \amp = 1+(-x^{2})+(-x^{2})^{2}+(-x^{2})^{3}+\cdots</mrow>
                        <mrow> \amp = 1-\dfrac{x^{2}}{2!} +\dfrac{x^{4}}{4!}-\cdots</mrow>
                        <mrow> \amp = \sum_{k=0}^{\infty}(-1)^{k}x^{2k}</mrow>
                    </md></p>
                   <p> which will converge on the interval <m>\lvert -x^{2}\rvert &lt; 1, </m> i.e., <m> -1&lt; x &lt; 1. </m>  </p>
                </solution>
</example>
        
<example xml:id="Maclaurin_series_x_on_2_minus_5x">

            <p>Find the Maclaurin series for  <m> f(x)=\dfrac{1}{1+x^{2}}. </m> </p>
             <solution>
                    <p>Once again we will use the Maclaurin series for <m>f(x)=\dfrac{1}{1-x}</m> on <m>\lvert x\rvert &lt; 1. </m> Now </p>                 
                        <p><md>
                        <mrow> \frac{x^2}{2-5x} \amp =\dfrac{x^{2}}{2}(\dfrac{1}{1-(\frac{5x}{2})})</mrow>
                        <mrow> \amp = \dfrac{x^2}{2}(1+(\frac{5x}{2})+(\frac{5x}{2})^{2}+(\frac{5x}{2})^{3}+\cdots)</mrow>
                        <mrow> \amp = \dfrac{x^2}{2}\sum_{k=0}^{\infty}(\dfrac{5x}{2})^{k}</mrow>
                    </md></p>
                   <p> which will converge on the interval <m>\lvert \frac{5x}{2}\rvert &lt; 1, </m> i.e., <m> -\frac{2}{5}&lt; x &lt; \frac{2}{5}. </m>  </p>
                </solution>
</example>            
            
<example xml:id="Maclaurin_series_e_minus_x_2">

            <p>Find the Maclaurin series for  <m> f(x)=e^{-x^2}. </m> </p>
             <solution>
                    <p>Substituting into the Maclaurin series for  <m>f(x)=e^{x}</m> . </p>                 
                        <p><md>
                        <mrow>e^{-x^2} \amp =\sum_{k=0}^{\infty}\dfrac{(-x^2)^{k}}{k!}=\sum_{k=0}^{\infty}(-1)^{k}\dfrac{(x)^{2k}}{k!}</mrow>
                        <mrow> \amp = 1- x^{2}+\frac{x^{4}}{2!}-\frac{x^{6}}{3!}+\cdots</mrow>
                    </md></p>
                   <p> which will converge for all real values of <m> x. </m>  </p>
                </solution>
</example>           
       
            
<paragraphs><title>Differentiating/Integrating Known Series</title></paragraphs>         
<p> As the theorem below says, we can also use differentiation and integration to work out new Maclaurin series expansions from ones that we already know. The proof of this theorem is beyond the scope of this course.  </p>            
    
<theorem>
                <statement>
                    <p>
                      If  <m>f(x)=\sum\limits_{k=0}^{\infty}c_{k}x^{k}</m> with radius of convergence <m> \mathbb{R} </m> then                    </p>
                  <p><ol label="i">
            <li><p> <m>f'(x)=\sum\limits_{k=0}^{\infty}k c_{k}x^{k-1}</m> with radius of convergence   <m> \mathbb{R}, </m> </p></li>
            <li><p><m> \int f(x)dx=K+ \sum\limits_{k=0}^{\infty} \dfrac{c_{k}}{k+1}x^{k-1}</m> with radius of convergence   <m> \mathbb{R}, </m> (where <m> K </m>  is a constant). </p></li>
        </ol></p>
                </statement>
        </theorem>            
            
<p> Note that the behaviour of the series (i.e. whether it converges or diverges) at the endpoints may change when it is differentiated or integrated. </p>            
            
<example xml:id="Maclaurin_series_1_on_1_minus_x_power_2">

            <p>Find the Maclaurin series for  <m> ff(x)=\dfrac{1}{(1-x)^{2}}.</m> </p>
             <solution>
                    <p> Notice that <m>\int \frac{1}{(1-x)^{2}}=\frac{1}{1-x}, </m> or put the other way, <m> \frac{1}{(1-x)^{2}}=\frac{d}{dx} (\frac{1}{1-x}). </m> Since we know the Maclaurin series for <m> \frac{1}{1-x} </m> we can differentiate this series to obtain the Maclaurin series for <m> \frac{1}{(1-x)^{2}}. </m> So, on <m>\lvert x\rvert &lt; 1, </m>  </p>                 
                        <p><md>
                        <mrow> \frac{1}{(1-x)^{2}} \amp =\frac{d}{dx}(\sum_{k=0}^{\infty} x^{k})</mrow>            
                        <mrow> \amp = \frac{d}{dx}(\sum_{k=1}^{\infty} k x^{k-1}</mrow>
                        <mrow> \amp = 1+2x+3x^2+4x^3+\dots </mrow>
                    </md></p>
                </solution>
</example>

              
<example xml:id="Maclaurin_series_ln_1_plus_x">

            <p>Find the Maclaurin series for  <m> ff(x)=\ln(1+x).</m> </p>
             <solution>
                    <p> Notice that <m> \frac{d}{(dx)}(\ln(1+x)), </m> or put the other way, <m> \ln(1+x)=K+\int \frac{1}{1+x}. </m> Since we know the Maclaurin series for <m> \frac{1}{1+x} </m> we can integrate this series to obtain the Maclaurin series for <m> \ln(1+x).</m> So, on <m>\lvert x\rvert &lt; 1, </m>  </p>                 
                        <p><md>
                        <mrow> \ln(1+x) \amp = K+\int (\sum_{k=0}^{\infty} (-x)^{k})dx</mrow>            
                        <mrow> \amp = K+\sum_{k=0}^{\infty} (-1)^{k}\frac{x^{k+1}}{k+1}</mrow>
                        <mrow> \amp = K + x - \frac{1}{2}x^{2} +\frac{1}{3}x^{3} - \dots</mrow>
                    </md></p>
                    <p> Since <m> \ln(1+x)</m> is <m> 0 </m> when <m> x=0 </m> we have <m> K=0. </m> Thus on <m>\lvert x\rvert &lt; 1 </m> </p>
                     <me>  \ln(1+x)=\sum_{k=0}^{\infty}(-1)^{k-1}\frac{x^{k}}{k}=x-\frac{x^{2}}{2}+\frac{x^{3}}{3}-\cdots \cdot </me>
                </solution>
</example>


        <exercises>
            <title>Example Tasks</title>

            <exercise> 
                <statement>
                    <p> Find the Maclaurin series for  <m> f(x)=\frac{1}{3+2x}. </m> </p>
                </statement>
            </exercise>
             
                <exercise> 
                <statement>
                    <p> Find the Maclaurin series for  <m> f(x)=\frac{1-x^2}{5-3x^2}. </m> </p>
                </statement>
            </exercise>
            
                <exercise> 
                <statement>
                    <p>  Find the Maclaurin series for <m> f(x)=\frac{1}{(1-2x)^2}. </m> </p>
                </statement>
            </exercise>

                <exercise> 
                <statement>
                    <p> Find the Maclaurin series for <m> f(x)=\tan{-1}(x). </m> </p>
                </statement>
            </exercise>
            
                            <exercise> 
                <statement>
                    <p> Use a sixth degree Maclaurin polynomial to estimate  <m> f(x)=\int_{0}^{1}e^{-x^{2}}dx. </m> </p>
                </statement>
            </exercise>
            
            
        </exercises>
     </section>
     
     
     
           <section xml:id="Taylor_Series">
            <title>Taylor Series</title>  
            
 <p >Maclaurin series are power series about <m> x=0. </m>  However we can follow exactly the same process to find a power series expansion for a function   <m> f(x) </m> about any point   <m> x=a. </m>  We call these power series Taylor Series. </p>
            

                      <definition>
            <title>Taylor Series</title>
            <statement>
                <p>The series, </p>
                 <p>   <me>\sum_{k=0}^{\infty}\dfrac{f^{(k)}(a)}{k!}=f(a)+f'(a)(x-a)+\dfrac{f''(a)}{2!}(x-a)^{2}+\dfrac{f'''(a)}{3!}(x-a)^3+ \dots </me>.</p>
                <p>is called the Taylor series for <m> f(x) </m> about   <m> x=a. </m>  </p>
            </statement>
        </definition>
            
 <p > Note that: </p>
 <p >
<ol >
<li > We can construct the Taylor series about  <m>x=a.  </m>  for any function that is infinitely differentiable at  <m>x=a.  </m> </li >
<li >
<p >
The Taylor series for <m> f </m> about  <m> x=a </m>    always converges to  at  <m> x=a. </m>  
</p >
</li >
 <li >
<p >
If the Taylor series converges for other values of <m> x </m> these will be in an interval centred on <m> x=a. </m>
</p >
</li >
 <li >
<p >
It is possible that a Taylor series may converge to a value other than the function value. 
</p >
</li >
 <li >
<p >
A Maclaurin series is just a Taylor series about  <m>x=0.  </m> 
 </p >
</li >
<li >
<p >
The <m> n^{\text{th}} </m>  partial sum of the Taylor series for <m> f </m> about <m> x=a </m>  is called the <m> n^{\text{th}} </m> degree Taylor polynomial for<m> f </m> about  <m> x=a. </m>
</p >
</li >
</ol >
</p >              
      
      <example xml:id="Taylor_series_cos">

            <p>Find the Taylor series for   <m> f(x)=\cos(x) </m> about <m> x=\frac{\pi}{2} </m>  </p>
             <solution>
                    <p> In order to find the Taylor series for   <m> f(x)=\cos(x) </m> about <m> x=\frac{\pi}{2} </m>   we need to evaluate <m> f </m> and its derivatives at  <m> x=\frac{\pi}{2}. </m>  So,  </p>
                    <p><md>
                       <mrow> f(x) \amp =\cos(x)  \,\, \text{and hence}\,\,   f(\frac{\pi}{2})=0  </mrow>           
                        <mrow> f'(x) \amp =\sin(x)  \,\, \text{and hence}\,\,   f'(\frac{\pi}{2})=-1 </mrow>
                        <mrow> f''(x) \amp =-\cos(x)  \,\, \text{and hence}\,\,   f''(\frac{\pi}{2})=0  </mrow>
                         <mrow> f'(x) \amp =-\sin(x)  \,\, \text{and hence}\,\,   f'''(\frac{\pi}{2})=1 </mrow>
                         <mrow>\amp \hspace{5.5cm}  \vdots </mrow>
                          <mrow>\amp \hspace{4.6cm}  f^{(k)}(\frac{\pi}{2})=\begin{cases} 0 \amp k\;\, \text{even} \\
           (-1)^{\frac{k+1}{2}} \amp  k \;\, \text{odd} \end{cases} </mrow>
                    </md></p>
                    <p> Thus the Taylor series for  <m> f(x)=\cos(x) </m> about <m> x=\frac{\pi}{2} </m>  is </p>
<p><md>
                        <mrow>  \amp = 0-(x-\frac{\pi}{2})+0+\frac{1}{3!}(x-\frac{\pi}{2})^{3}-\frac{1}{5!}(x-\frac{\pi}{2})^{5}+\dots</mrow>            
                        <mrow> \amp =-(x-\frac{\pi}{2})+\frac{(x-\frac{\pi}{2})^{3}}{3!}-\frac{(x-\frac{\pi}{2})^{5}}{5!}+\dots</mrow>
                        <mrow> \amp = \sum_{k=1}^{\infty}(-1)^{k}\dfrac{(x-\frac{\pi}{2})^{2k-1}}{(2k-1)!}.</mrow>
                    </md></p>
                  <p> It turns out that this series converges to  <m> f(x)=\cos(x) </m> for all values of <m> x. </m>  <xref ref="Fig-Taylor_series_cos"/> shows the graph of <m> f(x)=\cos(x) </m> and the Taylor polynomials of degree <m> 1 </m>  and degree <m>  3    </m> about <m> x=\frac{\pi}{2} .</m>   </p>
                     <figure xml:id="Fig-Taylor_series_cos">
                <caption></caption>
                <image source="./Calculus/Images/2/Taylor_series_cos.png" width="85%"/>
            </figure>
                </solution>
</example>              
        
        
        
    <example xml:id="Second_order_approximation_e_power_minus_x_on_3">

            <p>Find the second order approximation to   <m> f(x)=e^{-\frac{x}{3}} </m> about <m> x=2. </m>  </p>
             <solution>
                    <p> In order to find the second order approximation for <m> f(x)=e^{-\frac{x}{3}} </m> about <m> x=2 </m> we need to evaluate <m> f </m> and its first two derivatives at <m> x=2. </m> .  So,  </p>                 
                        <p><md>
                        <mrow> f(x) \amp =e^{-\frac{x}{3}}  \,\, \text{and hence}\,\,   f(2)=e^{-\frac{2}{3}}  </mrow>           
                        <mrow> f'(x) \amp =-\frac{1}{3}e^{-\frac{x}{3}}  \,\, \text{and hence}\,\,   f'(2)=-\frac{1}{3}e^{-\frac{2}{3}} </mrow>
                        <mrow> f''(x) \amp =\frac{1}{9}e^{-\frac{x}{3}}  \,\, \text{and hence}\,\,   f''(2)=\frac{1}{9}e^{-\frac{2}{3}}   </mrow>
                        </md></p>
                    <p> Thus the second order approximation for <m> f(x)=e^{-\frac{x}{3}} </m> about <m> x=2, </m> (or the Taylor polynomial of degree <m> 2, </m> for <m> f(x)=e^{-\frac{x}{3}} </m> about <m> x=2, </m>), is </p>
                   <p><md>
                        <mrow> T_{2}(x) \amp =e^{-\frac{2}{3}}-\frac{1}{3}e^{-\frac{2}{3}}(x-2)+\frac{1}{9}e^{-\frac{2}{3}}\dfrac{(x-2)^{2}}{2}  </mrow>           
                        <mrow> \amp =e^{-\frac{2}{3}}-\frac{1}{3}e^{-\frac{2}{3}}(x-2)+\frac{1}{18}e^{-\frac{2}{3}}(x-2)^{2} </mrow>
                        </md></p>
                </solution>
</example>
            
 <example xml:id="Fourth_order_approximation_e_power_minus_x_on_3">

            <p> Find the Taylor polynomial of degree <m> 4 </m> for <m> f(x)=x\cos(x) </m>  about <m> x=\frac{\pi}{2}. </m>  </p>
             <solution>
                    <p> Since we already know the Taylor series for  <m> \cos(x) </m>  about  <m> x=\frac{\pi}{2}  </m>   we can obtain the <m> 4^{\text{th}} </m> degree Taylor polynomial for <m> f(x)=x\cos(x) </m> about <m> x=\frac{\pi}{2}. </m> as follows </p>                 
                        <p><md>
                        <mrow> f(x) \amp = x\cos(x)  </mrow>           
                        <mrow>  \amp = (x-\frac{\pi}{2})\cos(x)+\frac{\pi}{2}\cos(x) </mrow>
                        <mrow>   \amp = (x-\frac{\pi}{2})  \big[-(x-\frac{\pi}{2}) + \frac{(x-\frac{\pi}{2})^3}{3!} -  \frac{(x-\frac{\pi}{2})^5}{5!} + \dots   \big] + \frac{\pi}{2}\big[ -(x-\frac{\pi}{2}) +  \frac{(x-\frac{\pi}{2})^3}{3!} -  \frac{(x-\frac{\pi}{2})^5}{5!} + \dots   \big] </mrow>
                        <mrow>   \amp = \big[-(x-\frac{\pi}{2})^2 + \frac{(x-\frac{\pi}{2})^4}{3!} - \dots   \big] + \big[ -\frac{\pi}{2}(x-\frac{\pi}{2}) + \frac{\pi}{2}\frac{(x-\frac{\pi}{2})^3}{3!} - \dots   \big]. </mrow>
                        </md></p>
                    <p> Thus the <m> 4^{\text{th}} </m> degree Taylor polynomial is </p>
                   <p><me>
                      T_{4}(x) = -\frac{\pi}{2}  (x-\frac{\pi}{2}) -  (x-\frac{\pi}{2})^2 +  \frac{\pi}{2} \frac{(x-\frac{\pi}{2})^3}{3!}  + \frac{(x-\frac{\pi}{2})^4}{3!}.   
                        </me></p>
                </solution>
</example>
            
              <exercises>
            <title>Example Tasks</title>

            <exercise> 
                <statement>
                    <p> Find the Taylor series for  <m> f(x)=\ln(x). </m> about <m> x=e. </m> </p>
                </statement>
            </exercise>
             
                <exercise> 
                <statement>
                    <p> Find the Taylor polynomial of degree  <m> 3 </m> for   <m> f(x)=\frac{1}{1-x} </m> about <m> x=2. </m>  </p>
                </statement>
            </exercise>
            
                <exercise> 
                <statement>
                    <p> Find the Taylor polynomial of degree  <m> 4 </m> for   <m> f(x)=x\ln(x) </m> about <m> x=e. </m>  </p>
                </statement>
            </exercise>

                <exercise> 
                <statement>
                    <p>  Find the Taylor polynomial of degree  <m> 3  </m> for   <m> f(x)=x^2 e^{x} </m> about <m> x=1. </m>  </p>
                </statement>
            </exercise>
 </exercises>
             <remark>
            <title>A little remark</title>
                <p>
                    Computer algebra systems usually have commands for Taylor series. For example, here in <xref ref="Fig-Taylor_series_cos_Mathematica"/> is an example of a query to Wolfram Alpha that will work.
                </p>
                <figure xml:id="Fig-Taylor_series_cos_Mathematica">
                    <image source="./Calculus/Images/2/Taylor_series_cos_Mathematica.png" width="90%"/>
                </figure>
            </remark>
            
            
            
            

        </section>
<!-- =================================================================================================== -->
</chapter>